src/decode.v
@@ -1,0 +1,291 @@
+Require Import Coq.Arith.Arith.
+Require Import Coq.omega.Omega.
+Require Import Lists.List.
+Import ListNotations.
+
+Require ast.
+
+(* Helpers *)
+
+Notation "'do' '(' a ',' b ')' '<-' e ';' c" :=
+  (match e with | None => None | Some (a, b) => c end)
+    (at level 70, right associativity).
+
+Definition stream := list bool.
+
+Fixpoint number_rec (bits: nat) (s: stream) (acc: N):
+  option (N * stream) :=
+  match bits, s with
+  | 0, _ => Some (acc, s)
+  | _, nil => None
+  | (S bits), (cons bit s) =>
+    number_rec bits s
+               (N.lor acc (N.shiftl (N.b2n bit) (N.of_nat bits)))
+  end.
+
+Lemma number_rec_some:
+  forall (bits: nat) (s: stream) (acc: N),
+    (List.length s >= bits) ->
+    exists (r: N * stream),
+      (number_rec bits s acc) = Some r.
+Proof.
+  induction bits; intros.
+  - exists (acc, s). trivial.
+  - simpl. case_eq s; intros; subst.
+    + contradict H. simpl. omega.
+    + apply IHbits.
+      simpl in H.
+      omega.
+Qed.
+
+Lemma number_rec_skipn:
+  forall (bits: nat) (s: stream) (acc: N) (n: N) (s': stream),
+    (number_rec bits s acc) = Some (n, s') ->
+    s' = skipn bits s.
+Proof.
+  induction bits; intros.
+  - compute in H. injection H.
+    intros. simpl. rewrite H0. reflexivity.
+  - destruct s; simpl in H.
+    + contradict H. discriminate.
+    + apply IHbits in H. simpl. assumption.
+Qed.
+
+Lemma size_lor: forall(a b: N)(s: nat),
+    N.size_nat a <= s ->
+    N.size_nat b <= s ->
+    N.size_nat (N.lor a b) <= s.
+Proof. Admitted.
+
+Lemma number_rec_bits_acc:
+  forall (bits: nat) (s: stream) (acc: N) (n: N) (s': stream),
+    (number_rec bits s acc) = Some (n, s') ->
+    (N.size_nat n <= bits + N.size_nat acc).
+Proof.
+  induction bits; intros.
+  - compute in H. injection H. intros.
+    rewrite H1. omega.
+  - destruct s; simpl in H.
+    + discriminate.
+    + pose (complik := (N.lor acc (N.shiftl (N.b2n b) (N.of_nat bits)))).
+      specialize IHbits with (s) (complik) (n) (s').
+      apply IHbits in H.
+      apply Nat.le_trans with (m:=bits + N.size_nat complik).
+      assumption.
+      simpl. rewrite plus_n_Sm.
+      apply plus_le_compat_l.
+      unfold complik. unfold complik in H.
+      apply size_lor; try omega.
+      destruct b; subst. simpl; simpl in H.
+Admitted.
+
+Lemma number_rec_bits:
+  forall (bits: nat) (s: stream) (s': stream) (n: N),
+    (number_rec bits s 0) = Some (n, s') ->
+    (N.size_nat n <= bits).
+Proof.
+  intros.
+  specialize number_rec_bits_acc with (bits)(s)(0%N)(n)(s').
+  intros.
+  apply H0 in H.
+  rewrite Nat.add_comm in H.
+  simpl in H.
+  assumption.
+Qed.
+
+Definition number (bits: nat) (s: stream):
+  option (N * stream) := (number_rec bits s 0).
+
+Lemma skipn_length {A}: forall (n: nat)(l: list A),
+    List.length (List.skipn n l) <= List.length l.
+Proof.
+  induction n.
+  - trivial.
+  - destruct l.
+    + trivial.
+    + simpl. specialize IHn with (l). omega.
+Qed.
+
+Lemma number_consumes:
+  forall (bits: nat) (s s': stream) (n: N),
+    number (S bits) s = Some (n, s') ->
+    List.length s' < List.length s.
+Proof.
+  intros.
+  unfold number in H.
+  specialize number_rec_skipn with ((S bits))(s)(0%N)(n)(s').
+  intros.
+  assert (s' = skipn (S bits) s). {
+    apply H0. apply H.
+  }
+  subst.
+  induction s.
+  - contradict H. simpl. discriminate.
+  - simpl.
+    apply le_lt_n_Sm.
+    apply skipn_length.
+Qed.
+
+Definition expect (bits: nat) (expected: N) (s: stream):
+  option (unit * stream) :=
+  do (n, s) <- (number bits s);
+    if (N.eqb n expected)
+    then Some (tt, s)
+    else None.
+
+(* Actual Code *)
+
+Definition condition (s: stream):
+  option (ast.condition * stream) :=
+  do (n, s) <- (number 4 s);
+  match n with
+  | 0%N => Some (ast.none, s)
+  | 1%N => Some (ast.le, s)
+  | 2%N => Some (ast.l, s)
+  | 3%N => Some (ast.e, s)
+  | 4%N => Some (ast.ne, s)
+  | 5%N => Some (ast.ge, s)
+  | 6%N => Some (ast.g, s)
+  | _ => None
+  end.
+
+(* TODO: whatappenz with invalid values *)
+
+Definition register (s: stream): option (ast.register * stream) :=
+  do (n, s) <- (number ast.register_bits s);
+  Some (ast.reg n, s).
+
+Definition immediate (s: stream): option (ast.immediate * stream) :=
+  do (n, s) <- (number ast.constant_bits s);
+  Some (ast.imm n, s).
+
+Definition displacement (s: stream): option (ast.displacement * stream) :=
+  do (n, s) <- (number ast.constant_bits s);
+  Some (ast.dsp n, s).
+
+Definition destination (s: stream): option (ast.destination * stream) :=
+  do (n, s) <- (number ast.constant_bits s);
+  Some (ast.dst n, s).
+
+(* Actual instruction decoding *)
+
+Definition rrmovl (s: stream): option (ast.instruction * stream) :=
+  do (cond, s) <- (condition s);
+  do (reg1, s) <- (register s);
+  do (reg2, s) <- (register s);
+  Some (ast.rrmovl cond reg1 reg2, s).
+
+Definition irmovl (s: stream): option (ast.instruction * stream) :=
+  (* 15 is 0x0F, it's required by the spec *)
+  do (n, s) <- (expect 8 15 s);
+  do (reg1, s) <- (register s);
+  do (val, s) <- (immediate s);
+  Some (ast.irmovl val reg1, s).
+
+Definition rmmovl (s: stream): option (ast.instruction * stream) :=
+  do (n, s) <- (expect 4 0 s);
+  do (reg1, s) <- (register s);
+  do (reg2, s) <- (register s);
+  do (val, s) <- (displacement s);
+  Some (ast.rmmovl reg1 val reg2, s).
+
+Definition mrmovl (s: stream): option (ast.instruction * stream) :=
+  do (n, s) <- (expect 0 4 s);
+  do (reg1, s) <- (register s);
+  do (reg2, s) <- (register s);
+  do (val, s) <- (displacement s);
+  Some (ast.mrmovl val reg1 reg2, s).
+
+Definition op (s: stream): option (ast.operator * stream) :=
+  do (n, s) <- (number 4 s);
+  match n with
+  | 0%N => Some (ast.addl, s)
+  | 1%N => Some (ast.subl, s)
+  | 2%N => Some (ast.andl, s)
+  | 3%N => Some (ast.xorl, s)
+  | _ => None
+  end.
+
+Definition OPl (s: stream): option (ast.instruction * stream) :=
+  do (op, s) <- (op s);
+  do (reg1, s) <- (register s);
+  do (reg2, s) <- (register s);
+  Some (ast.OPl op reg1 reg2, s).
+
+Definition jump (s: stream): option (ast.instruction * stream) :=
+  do (cond, s) <- (condition s);
+  do (dest, s) <- (destination s);
+  Some (ast.jump cond dest, s).
+
+Definition ret (s: stream): option (ast.instruction * stream) :=
+  do (n, s) <- (expect 0 4 s);
+  Some (ast.ret, s).
+
+Definition pushl (s: stream): option (ast.instruction * stream) :=
+  do (n, s) <- (expect 0 4 s);
+  do (reg1, s) <- (register s);
+  do (n, s) <- (expect 15 4 s);
+  Some (ast.pushl reg1, s).
+
+Definition popl (s: stream): option (ast.instruction * stream) :=
+  do (n, s) <- (expect 0 4 s);
+  do (reg1, s) <- (register s);
+  do (n, s) <- (expect 15 4 s);
+  Some (ast.popl reg1, s).
+
+Definition instruction (s: stream) : option (ast.instruction * stream) :=
+  do (n, s) <- (number 4 s);
+  match n with
+  | 0%N => do (_, s) <- (expect 0 4 s);
+           Some (ast.halt, s)
+  | 1%N => do (_, s) <- (expect 0 4 s);
+           Some (ast.nop, s)
+  | 2%N => rrmovl s
+  | 3%N => irmovl s
+  | 4%N => rmmovl s
+  | 5%N => mrmovl s
+  | 6%N => OPl s
+  | 7%N => jump s
+  | 8%N => rrmovl s
+  | 9%N => ret s
+  | 10%N => pushl s
+  | 11%N => popl s
+  | _ => None
+  end.
+
+Lemma instruction_consumes:
+  forall (s s': stream) (i: ast.instruction),
+    instruction s = Some (i, s') ->
+    List.length s' < List.length s.
+Proof.
+  intros.
+  unfold instruction, rrmovl, irmovl, rmmovl, mrmovl,
+  OPl, jump, rrmovl, ret, pushl, popl, register,
+  expect, immediate, displacement, destination in H.
+  case_eq (number 4 s); intros; rewrite H0 in H.
+Admitted.
+
+Require Coq.Program.Wf.
+Program Fixpoint _instructions_rec
+        (s: stream) (acc: ast.instructions)
+        {measure (List.length s)}: option (ast.instructions) :=
+  match s with
+  | nil => Some acc
+  | s => match instruction s with
+    | None => None
+    | Some (instr, s) => _instructions_rec s (cons instr acc)
+    end
+  end.
+Next Obligation.
+  apply
+
+(*Fixpoint _get_instructions_rec (bits: stream) (acc: instructions): option (instructions) :=
+  match bits with
+  | nil => Some acc
+  | bits => match decode bits with
+    | None => None
+    | Some (instr, s) => _get_instructions_rec s (cons instr acc)
+    end
+  end.*)
+
+Definition instructions (bits: stream): option (ast.instructions) := _instructions_rec bits nil.
