src/encode.v
@@ -1,0 +1,135 @@
+Require Import Coq.Arith.Arith.
+Require Import Coq.omega.Omega.
+Require Import Lists.List.
+Import ListNotations.
+
+Require ast.
+
+Fixpoint number_rec
+         (n: N) (bits: nat) (acc: list bool): list bool :=
+  match bits with
+  | 0 => acc
+  | S b => number_rec
+             (N.shiftr n 1) b (cons (N.testbit n 0) acc)
+  end.
+
+(* Encodes a number into binary (little endian) *)
+Definition number (bits: nat) (n: N): list bool :=
+  number_rec n bits nil.
+
+Lemma number_rec_bits:
+  forall (bits: nat) (n: N) (acc: list bool),
+    List.length (number_rec n bits acc)
+    = (List.length acc) + bits.
+Proof.
+  induction bits; intros.
+  - trivial.
+  - simpl.
+    rewrite <- plus_n_Sm.
+    apply IHbits.
+Qed.
+
+Lemma number_bits: forall (n: N)(bits: nat),
+    List.length (number bits n) = bits.
+Proof.
+  intros.
+  unfold number. simpl. rewrite number_rec_bits.
+  compute. trivial.
+Qed.
+
+Notation "'b[' n ';' b ']'" := (number b n) (at level 60).
+
+Goal b[0; 4] = [false; false; false; false].
+Proof. trivial. Qed.
+Goal b[5; 4] = [false; true; false; true].
+Proof. trivial. Qed.
+Goal b[15; 4] = [true; true; true; true].
+Proof. trivial. Qed.
+
+Definition operator_num (op: ast.operator): N :=
+  match op with
+  | ast.addl => 0
+  | ast.subl => 1
+  | ast.andl => 2
+  | ast.xorl => 3
+  end.
+
+Fact operator_4bits (op: ast.operator):
+  (N.size_nat (operator_num op)) <= 4.
+Proof. case op; compute; omega. Qed.
+
+Definition operator (op: ast.operator): list bool :=
+  (number 4 (operator_num op)).
+
+Definition condition_num (cond: ast.condition): N :=
+  match cond with
+  | ast.none => 0
+  | ast.le => 1
+  | ast.l => 2
+  | ast.e => 3
+  | ast.ne => 4
+  | ast.ge => 5
+  | ast.g => 6
+  end.
+
+Fact condition_4bits (cond: ast.condition):
+  N.size_nat (condition_num cond) <= 4.
+Proof. case cond; compute; omega. Qed.
+
+Definition condition (cond: ast.condition): list bool :=
+  (number 4 (condition_num cond)).
+
+Definition register (r: ast.register): list bool :=
+  match r with
+  | ast.reg n => (number ast.register_bits n)
+  end.
+
+Definition immediate (i: ast.immediate): list bool :=
+  match i with
+  | ast.imm n => (number ast.constant_bits n)
+  end.
+
+Definition displacement (d: ast.displacement): list bool :=
+  match d with
+  | ast.dsp n => (number ast.constant_bits n)
+  end.
+
+Definition destination (d: ast.destination): list bool :=
+  match d with
+  | ast.dst n => (number ast.constant_bits n)
+  end.
+
+Definition instruction (i: ast.instruction): list bool :=
+  match i with
+  | ast.halt => b[0; 4] ++ b[0; 4]
+  | ast.nop => b[1; 4] ++ b[0; 4]
+  | ast.rrmovl cond ra rb =>
+    b[2; 4] ++ (condition cond) ++ (register ra) ++ (register rb)
+  | ast.irmovl v rb =>
+    b[3; 4] ++ b[0; 4] ++ b[15; 4] ++ (register rb) ++ (immediate v)
+  | ast.rmmovl ra d rb =>
+    b[4; 4] ++ b[0; 4] ++ (register ra) ++ (register rb) ++ (displacement d)
+  | ast.mrmovl d ra rb =>
+    b[5; 4] ++ b[0; 4] ++ (register ra) ++ (register rb) ++ (displacement d)
+  | ast.OPl op ra rb =>
+    b[6; 4] ++ (operator op) ++ (register ra) ++ (register rb)
+  | ast.jump cond d =>
+    b[7; 4] ++ (condition cond) ++ (destination d)
+  | ast.call d =>
+    b[8; 4] ++ b[0; 4] ++ (destination d)
+  | ast.ret => b[9; 4] ++ b[0; 4]
+  | ast.pushl ra =>
+    b[10; 4] ++ b[0; 4] ++ (register ra) ++ b[15; 4]
+  | ast.popl ra =>
+    b[11; 4] ++ b[0; 4] ++ (register ra) ++ b[15; 4]
+  end.
+
+Fixpoint instructions_rev (ins: ast.instructions): list bool :=
+  match ins with
+  | cons i ins => List.rev_append (instruction i)
+                                  (instructions_rev ins)
+  | nil => nil
+  end.
+
+Definition instructions (ins: ast.instructions): list bool :=
+  List.rev (instructions_rev ins).
