Makefile
@@ -3,3 +3,7 @@ all: build
 .PHONY: build
 build:
 	coqtop -color yes -I src -compile src/ast.v
+
+.PHONY: clean
+clean:
+	rm -f src/*.aux src/*.glob src/*.vo
